\ifx\wholebook\relax \else
% ------------------------

\documentclass[UTF8]{article}
%------------------- Other types of document example ------------------------
%
%\documentclass[twocolumn]{IEEEtran-new}
%\documentclass[12pt,twoside,draft]{IEEEtran}
%\documentstyle[9pt,twocolumn,technote,twoside]{IEEEtran}
%
%-----------------------------------------------------------------------------
\input{../../../common-en.tex}

\setcounter{page}{1}

\begin{document}

%--------------------------

% ================================================================
%                 COVER PAGE
% ================================================================

\title{Proof of AVL tree pattern matching algorithm}

\author{Larry~LIU~Xinyu
\thanks{{\bfseries Larry LIU} \newline
  Email: liuxinyu95@gmail.com \newline}
  }

\maketitle
\fi

\markboth{Proof of AVL tree}{Elementary Algorithms}

\ifx\wholebook\relax
\chapter{Proof of AVL tree pattern matching algorithm}
\numberwithin{Exercise}{chapter}
\fi

% ================================================================
%                 Introduction
% ================================================================

This appendix provides proofs to result we uses in the AVL tree pattern
matching insert algorithm.

\section{Height increment after insertion}

When insert a key to the AVL tree, the increment to the height can be deduced
into four cases given as below.

\[
\begin{array}{rl}
  \Delta H & = |T'| - |T| \\
              & = \left \{
                  \begin{array}{r@{\quad:\quad}l}
                  \Delta H_r & \Delta \geq 0 \land \Delta' \geq 0 \\
                  \Delta + \Delta H_r & \Delta \leq 0 \land \Delta' \geq 0 \\
                  \Delta H_l - \Delta & \Delta \geq 0 \land \Delta' \leq 0 \\
                  \Delta H_l & otherwise
                  \end{array} \right .
\end{array}
\]

To prove this equation, note the fact that the height can't increase
both in left and right with only one insertion.

These 4 cases can be explained from the balance factor
definition that it equals to the difference of the right and left sub trees.

\begin{itemize}
\item If $\Delta \geq 0$ and $\Delta' \geq 0$, it means that the height
of right sub tree isn't less than the left sub tree
before and after insertion. In this case, the increment in
height of the tree only is `contributed' from the right sub tree, which
is $\Delta H_r$.

\item If $\Delta \leq 0$, it means the height of left sub tree isn't
less than the right before. Since $\Delta' \geq 0$ after insertion,
we know the height of right sub tree increases,
and the left side keeps same ($|T_l'|=|T_l|$). The increment in height is
as the following.

\[
\begin{array}{rll}
\Delta H & = max(|T_r'|, |T_l'|) - max (|T_r|, |T_l|) & \{\Delta \leq 0 \land \Delta' \geq 0 \}\\
         & = |T_r'|-|T_l| & \{|T_l|=|T_l'| \}\\
         & = |T_r|+\Delta H_r - |T_l| & \\
         & = \Delta + \Delta H_r &
\end{array}
\]

\item For the case $\Delta \geq 0$ and $\Delta' \leq 0$, similar as the
above one, we can get the below result.

\[
\begin{array}{rll}
\Delta H & = max(|T_r'|, |T_l'|) - max (|T_r|, |T_l|) & \{\Delta \geq 0 \land \Delta' \leq 0 \}\\
         & = |T_l'|-|T_r| & \\
         & = |T_l|+\Delta H_l - |T_r| & \\
         & = \Delta H_l - \Delta&
\end{array}
\]

\item For the last case, both $\Delta$ and $\Delta'$ are no bigger than
zero. It means the height of left sub tree is always greater than or equal
 to the right. The increment in height is only `contributed'
from the left sub tree, which is $\Delta H_l$.
\end{itemize}


\section{Proof to the balance adjustment after insertion}

Given the 4 cases need fix as shown in figure \ref{fig:avl-insert-fix}, The balance factors are either -2, or +2. After adjustment, the factor resumes
to 0. The left and right sub trees have the same height.

\begin{figure}[htbp]
   \begin{center}
     \setlength{\unitlength}{1cm}
     \begin{picture}(15, 15)
        % arrows
        \put(4.5, 9.5){\vector(1, -1){1}}
        \put(4.5, 5){\vector(1, 1){1}}
        \put(10, 9.5){\vector(-1, -1){1}}
        \put(10, 5){\vector(-1, 1){1}}
        % delta values
        \put(5, 13){$\delta(z) = -2$}
        \put(2.5, 12){$\delta(y) = -1$}
        \put(10, 13){$\delta(x) = 2$}
        \put(11.5, 11.5){$\delta(y) = 1$}
        \put(1.5, 5.5){$\delta(z) = -2$}
        \put(3.5, 4){$\delta(x) = 1$}
        \put(12, 5.5){$\delta(x) = 2$}
        \put(10.5, 4){$\delta(z) = -1$}
        \put(7.5, 10){$\delta'(y) = 0$}
        % graphics
	\put(0, 7){\includegraphics[scale=0.5]{../../../datastruct/tree/AVL-tree/img/avl-insert-ll.ps}}
        \put(0, 0){\includegraphics[scale=0.5]{../../../datastruct/tree/AVL-tree/img/avl-insert-lr.ps}}
        \put(7, 7){\includegraphics[scale=0.5]{../../../datastruct/tree/AVL-tree/img/avl-insert-rr.ps}}
        \put(8.5, 0){\includegraphics[scale=0.5]{../../../datastruct/tree/AVL-tree/img/avl-insert-rl.ps}}
        \put(2, 5){\includegraphics[scale=0.5]{../../../datastruct/tree/AVL-tree/img/avl-insert-fixed.ps}}
      \end{picture}
     \caption{4 cases for balancing a AVL tree after insertion} \label{fig:avl-insert-fix-appendix}
  \end{center}
\end{figure}

These four cases are left-left lean, right-right lean, right-left lean,
and left-right lean cases. We denote
the balancing factor before fixing as $\delta(x), \delta(y)$, and $\delta(z)$, while after fixing, they changes to $\delta'(x), \delta'(y)$, and
$\delta'(z)$ respectively.

We'll next prove that, after fixing, we have $\delta(y)=0$ for all
four cases, and we'll provide the result values of $\delta'(x)$ and
$\delta'(z)$.

\subsubsection*{Left-left lean case}

As the structure of sub tree $x$ doesn't change due to fixing, we immediately get
$\delta'(x) = \delta(x)$.

Since $\delta(y) = -1$ and $\delta(z) = -2$, we have

\be
  \begin{array}{l}
  \delta(y) = |C| - |x| = -1 \Rightarrow |C| = |x| - 1 \\
  \delta(z) = |D| - |y| = -2 \Rightarrow |D| = |y| - 2
  \end{array}
  \label{eq:ll-cd}
\ee

After fixing.

\be
  \begin{array}{rll}
  \delta'(z) & = |D| - |C| & \{ From (\ref{eq:ll-cd}) \}\\
             & = |y| - 2 - (|x| - 1) & \\
             & = |y| - |x| - 1 & \{  x \text{ is child of } y \Rightarrow |y|-|x| = 1\} \\
             & = 0 &
  \end{array}
  \label{eq:ll-delta-z}
\ee

For $\delta'(y)$, we have the following fact after fixing.

\be
  \begin{array}{rll}
  \delta'(y) & = |z| - |x| & \\
             & = 1 + max(|C|, |D|) - |x| & \{ \text{By (\ref{eq:ll-delta-z}), we have} |C| = |D|\} \\
             & = 1 + |C| - |x| & \{ \text{By (\ref{eq:ll-cd})}\} \\
             & = 1 + |x| - 1 - |x| & \\
             & = 0 &
  \end{array}
\ee

Summarize the above results, the left-left lean case adjust the balancing
factors as the following.

\be
  \begin{array}{l}
  \delta'(x) = \delta(x) \\
  \delta'(y) = 0 \\
  \delta'(z) = 0
  \end{array}
\ee

\subsubsection*{Right-right lean case}

Since right-right case is symmetric to left-left case, we can easily achieve the result balancing factors as

\be
  \begin{array}{l}
  \delta'(x) = 0 \\
  \delta'(y) = 0 \\
  \delta'(z) = \delta(z)
  \end{array}
  \label{eq:rr-result}
\ee

\subsubsection*{Right-left lean case}

First let's consider $\delta'(x)$. After balance fixing, we have.

\be
  \delta'(x) = |B| - |A|
  \label{eq:rl-dx}
\ee

Before fixing, if we calculate the height of $z$, we can get.

\be
  \begin{array}{rll}
  |z| & = 1 + max(|y|, |D|) &  \{ \delta(z) = -1 \Rightarrow |y| > |D|\} \\
      & = 1 + |y| & \\
      & = 2 + max(|B|, |C|)
  \end{array}
  \label{eq:rl-z}
\ee

While since $\delta(x) = 2$, we can deduce that.

\be
  \begin{array}{rll}
  \delta(x) = 2 & \Rightarrow |z| - |A| = 2 & \{ \text{By (\ref{eq:rl-z})} \}\\
                & \Rightarrow 2 + max(|B|, |C|) - |A| = 2 & \\
                & \Rightarrow max(|B|, |C|) - |A| = 0 &
  \end{array}
  \label{eq:rl-ca}
\ee

If $\delta(y) = 1$, which means $|C| - |B| = 1$, it means

\be
  max(|B|, |C|)= |C| = |B|+1
\ee

Take this into (\ref{eq:rl-ca}) yields

\be
  \begin{array}{ll}
  |B|+1-|A| = 0 \Rightarrow |B|-|A|= -1 & \{ \text{By (\ref{eq:rl-dx}) } \} \\
  \Rightarrow \delta'(x) = -1 &
  \end{array}
\ee

If $\delta(y) \neq 1$, it means $max(|B|, |C|) = |B|$, taking this into
(\ref{eq:rl-ca}), yields.

\be
  \begin{array}{ll}
  |B| - |A| = 0  & \{ \text{By (\ref{eq:rl-dx})} \} \\
  \Rightarrow \delta'(x) = 0 &
  \end{array}
\ee

Summarize these 2 cases, we get relationship of $\delta'(x)$ and
$\delta(y)$ as the following.

\be
\delta'(x) = \left \{
  \begin{array}
  {r@{\quad:\quad}l}
  -1 & \delta(y) = 1 \\
  0 & otherwise
  \end{array}
\right.
\label{eq:rl-dx-dy}
\ee

For $\delta'(z)$ according to definition, it is equal to.

\be
  \begin{array}{rll}
    \delta'(z) & = |D| - |C| & \{ \delta(z) = -1 = |D| - |y| \} \\
               & = |y| - |C| - 1 & \{ |y| = 1 + max(|B|, |C|) \} \\
               & = max(|B|, |C|) - |C|
  \end{array}
  \label{eq:rl-dz}
\ee

If $\delta(y) = -1$, then we have $|C| - |B| = -1$, so $max(|B|, |C|) = |B| = |C| + 1$. Takes this into (\ref{eq:rl-dz}), we get $\delta'(z) = 1$.

If $\delta(y) \neq -1$, then $max(|B|, |C|) = |C|$, we get $\delta'(z)=0$.

Combined these two cases, the relationship between $\delta'(z)$ and $\delta(y)$ is as below.

\be
\delta'(z) = \left \{
  \begin{array}
  {r@{\quad:\quad}l}
  1 & \delta(y) = -1 \\
  0 & otherwise
  \end{array}
  \right.
  \label{eq:rl-dz-dy}
\ee

Finally, for $\delta'(y)$, we deduce it like below.

\be
  \begin{array}{rl}
  \delta'(y) & = |z| - |x| \\
             & = max(|C|, |D|) - max(|A|, |B|)
  \end{array}
  \label{eq:rl-dy}
\ee

There are three cases.
\begin{itemize}

\item If $\delta(y)=0$, it means $|B|=|C|$, and according to (\ref{eq:rl-dx-dy}) and (\ref{eq:rl-dz-dy}), we have $\delta'(x)=0 \Rightarrow |A| = |B|$, and $\delta'(z)=0 \Rightarrow |C|=|D|$, these lead to $\delta'(y)=0$.

\item If $\delta(y)=1$, From (\ref{eq:rl-dz-dy}), we have $\delta'(z)=0 \Rightarrow |C| = |D|$.
\[
  \begin{array}{rll}
  \delta'(y) & = max(|C|, |D|) - max(|A|, |B|) & \{|C|=|D|\} \\
             & = |C| - max(|A|, |B|) & \{\text{From (\ref{eq:rl-dx-dy}): $\delta'(x)=-1 \Rightarrow |B|-|A|=-1$} \} \\
             & = |C| - (|B| + 1) & \{ \delta(y) = 1 \Rightarrow |C|-|B|=1\} \\
             & = 0
  \end{array}
\]

\item If $\delta(y)=-1$, From (\ref{eq:rl-dx-dy}), we have $\delta'(x)=0 \Rightarrow |A|=|B|$.
\[
  \begin{array}{rll}
  \delta'(y) & = max(|C|, |D|) - max(|A|, |B|) & \{|A|=|B|\} \\
             & = max(|C|, |D|) - |B| & \{ \text{From (\ref{eq:rl-dz-dy}): $|D|-|C|=1$} \} \\
             & = |C| + 1 - |B| & \{  \delta(y) = -1 \Rightarrow |C|-|B|=-1\} \\
             & = 0
  \end{array}
\]

\end{itemize}

All three cases lead to the same result that $\delta'(y)=0$.

Collect all the above results, we get the new balancing factors after fixing as the following.

\be
  \begin{array}{l}
  \delta'(x) = \left \{
    \begin{array}
    {r@{\quad:\quad}l}
    -1 & \delta(y) = 1 \\
    0 & otherwise
    \end{array}
    \right. \\
  \delta'(y) = 0 \\
  \delta'(z) = \left \{
    \begin{array}
    {r@{\quad:\quad}l}
    1 & \delta(y) = -1 \\
    0 & otherwise
    \end{array}
    \right.
  \end{array}
  \label{eq:rl-result}
\ee

\subsubsection*{Left-right lean case}

Left-right lean case is symmetric to the Right-left lean case. By using
the similar deduction, we can find the new balancing factors are identical
to the result in (\ref{eq:rl-result}).

\ifx\wholebook\relax \else
%% \begin{thebibliography}{99}

%% \bibitem{CLRS}
%% Thomas H. Cormen, Charles E. Leiserson, Ronald L. Rivest and Clifford Stein.
%% ``Introduction to Algorithms, Second Edition''. ISBN:0262032937. The MIT Press. 2001

%% \end{thebibliography}

\end{document}
\fi
